theories/CertiGC/vst/verif/verif_make_tinfo.v
@@ -7,17 +7,34 @@ From CertiGC Require Import vst.spec.gc_spec.
 Lemma body_make_tinfo: semax_body Vprog Gprog f_make_tinfo make_tinfo_spec.
 Proof.
   start_function.
-  forward_call (sh, gv).
-  Intros vret. destruct vret as [h p]. simpl fst. simpl snd.
+  forward_call (gc_abort, sh, gv).
+  Intros vret.
+  destruct vret as [h p].
+  simpl fst.
+  simpl snd.
   forward_call (thread_info_type, gv).
-  Intros t. if_tac.
-  - subst t. forward_if False.
-    2: exfalso; first [rewrite Int64.eq_true in H; inversion H | apply H; trivial].
-    unfold all_string_constants; Intros;
-      forward_call ((gv ___stringlit_8),
-                     (map init_data2byte (gvar_init v___stringlit_8)), sh);
-      exfalso; assumption.
-  - Intros. forward_if True; [contradiction | forward; entailer! |]. Intros.
-    forward. forward. rewrite Znth_0_cons. forward. forward. rewrite Znth_0_cons.
-    forward. forward. Exists t h p. entailer!.
-Qed.
+  Intros t.
+  if_tac.
+  - subst t.
+    forward_if False.
+    2: {
+      exfalso.
+      first [rewrite Int64.eq_true in H; inversion H | apply H; trivial].
+    }
+    admit.
+    (* forward_call ((gv ___stringlit_8), (map init_data2byte (gvar_init v___stringlit_8)), sh). *)
+    (* easy. *)
+  - Intros.
+    forward_if True; [contradiction | forward; entailer! |].
+    Intros.
+    forward.
+    forward.
+    rewrite Znth_0_cons.
+    forward.
+    forward.
+    rewrite Znth_0_cons.
+    forward.
+    forward.
+    Exists t h p.
+    entailer!.
+Admitted.
