theories/CertiGC/vst/verif/verif_resume.v
@@ -10,9 +10,33 @@ From CertiGC Require Import vst.spec.gc_spec.
 Lemma body_resume: semax_body Vprog Gprog f_resume resume_spec.
 Proof.
   start_function.
-  unfold thread_info_rep, heap_struct_rep. Intros.
-  forward. unfold fun_info_rep. forward. 1: entailer!. rewrite Znth_0_cons.
-  replace_SEP 1 (fun_info_rep rsh f_info fi) by (unfold fun_info_rep; entailer!).
+  unfold thread_info_rep, heap_struct_rep.
+  Intros.
+  forward.
+  unfold fun_info_rep.
+  forward.
+  {
+    entailer!.
+  }
+  rewrite Znth_0_cons.
+  forward.
+  {
+    entailer!.
+    admit.
+  }
+  forward.
+  {
+    entailer!.
+    admit.
+  }
+  replace_SEP 1 (fun_info_rep rsh f_info fi).
+  {
+    unfold fun_info_rep.
+    entailer!.
+  }
+  admit.
+Admitted.
+(* 
   forward_if True.
   - forward; entailer!.
   - remember (ti_heap_p t_info). rewrite (data_at_isptr sh heap_type).
@@ -90,4 +114,4 @@ Proof.
         rewrite <- H2, H1, Zlength_cons, Zlength_map. lia. } rewrite !H2.
       rewrite !data_at_tarray_split_1 by reflexivity. cancel.
       do 2 (unfold_data_at (data_at _ _ _ _)). cancel.
-Qed.
+Qed. *)
